oik
git-svn-id: svn://scm.gforge.inria.fr/svn/cfml@204 ba02c806-7d2b-4818-9a48-35b22e6bdc79

imper/Loops.ml
@@ -1,4 +1,13 @@
 
+let myincr r =
+  r := !r + 1
+
+let incr_for k l =
+  for i = 1 to k do incr l done
+
+let incr_while k l =
+  while !k > 0 do incr l; decr k done
+
 (* todo: why body has type int->'a without annotation?*)
 
 let loop_for a b (body:int->unit) =
